ClickMG.v
@@ -35,8 +35,6 @@ Section TokenMG.
       try (left; reflexivity); try (right; discriminate).
   Defined.
 
-
-
   Inductive stage_place : token_transition -> token_transition -> Set :=
   (* L.ack -> L.req *)
   (* CLK- -> L.req *)
@@ -69,20 +67,72 @@ Section TokenMG.
   | right_ack_clk_rise : stage_place right_ack clk_rise
   .
 
-  Definition stage_MG : marked_graph token_transition :=
-    {| place := stage_place
-     ; init_marking := fun t1 t2 p => match p with
+
+  (** The only thing that is affected by token or non-token stages is the
+  initial markings. These are indexed by two boolean values: whether the current
+  stage has received a token or not on reset, and whether the current stage
+  generates a token or not on reset. *)
+
+Print marked_graph.
+
+  Definition init_marking_flag (in_flag : token_flag) (out_flag : token_flag) 
+      : forall t1 t2, stage_place t1 t2 -> nat :=
+    match in_flag, out_flag with
+    (* Traditional non-token stage *)
+    | Token, NonToken => fun t1 t2 p => match p with
                                       | left_req_clk_rise => 1
                                       | right_ack_clk_rise => 1
                                       | _ => 0
                                       end
+    (* Traditional token stage *)
+    | NonToken, Token => fun t1 t2 p => match p with
+                                      | right_req_left_req  => 1
+                                      | clk_fall_left_req   => 1
+                                      | left_ack_left_req   => 1
+                                      | right_req_right_ack => 1
+                                      | clk_fall_right_ack  => 1
+                                      | left_ack_right_ack  => 1
+                                      | _ => 0
+                                      end
+    (* Token with left token stage *)
+    | Token, Token    => fun t1 t2 p => match p with
+                                      | left_req_clk_rise => 1
+                                      | right_req_right_ack => 1
+                                      | clk_fall_right_ack  => 1
+                                      | left_ack_right_ack  => 1
+                                      | _ => 0
+                                      end
+    | NonToken, NonToken => fun t1 t2 p => match p with
+                                      | right_req_left_req  => 1
+                                      | clk_fall_left_req   => 1
+                                      | left_ack_left_req   => 1
+                                      | right_ack_clk_rise => 1
+                                      | _ => 0
+                                      end
+    end.
+
+  Variable in_flag out_flag : token_flag.
+
+  Definition stage_MG : marked_graph token_transition :=
+    {| place := stage_place
+     ; init_marking := init_marking_flag in_flag out_flag
      |}.
+
+End TokenMG.
+
+Existing Instance token_transition_eq_dec.
+
+Section SS_to_TokenMG.
 
   Variable even odd : Set.
   Context `{naming_scheme name even odd}.
   Variable dp_reset_n ctrl_reset_n : name.
 
   Variable l : latch even odd.
+  Variable in_flag : token_flag.
+  Definition out_flag := latch_to_token_flag l.
+      
+
 
   Definition transition_update_value (t : token_transition) (v : value) : value :=
     match t with
@@ -104,20 +154,7 @@ Section TokenMG.
   Definition transition_to_event (t : token_transition) (σ : state name) : event name value :=
     let x := transition_name t in
     Event x (transition_update_value t (σ x)).
-(*
-    match t with
-    | left_ack => let n := (ack (latch_input l))
-                  in Event n (neg_value (σ n))
-    | left_req => let n := (req (latch_input l))
-                  in Event n (neg_value (σ n))
-    | right_req => let n := (req (latch_output l))
-                   in Event n (neg_value (σ n))
-    | right_ack => let n := (ack (latch_output l))
-                   in Event n (neg_value (σ n))
-    | clk_rise  => Event (latch_clk l) Bit1
-    | clk_fall  => Event (latch_clk l) Bit0
-    end.
-*)
+
   Definition event_to_transition (e : event name value) : option token_transition :=
     match e with
     | Event x v => if x =? ack (latch_input l) then Some left_ack
@@ -142,60 +179,31 @@ Section TokenMG.
                                                  tail_list token_transition ->
                                                  Prop :=
   | equiv_t_empty : event_equiv_transition_trace t_empty t_empty
-(*
-  | equiv_left_ack t t' n v :
-    event_trace_equiv_transition_trace t t' ->
-    n = ack (latch_input l) ->
-    event_trace_equiv_transition_trace (t ▶ Event n v) (t' ▶ left_ack)
-  | equiv_left_req t t' n v :
-    event_trace_equiv_transition_trace t t' ->
-    n = req (latch_input l) ->
-    event_trace_equiv_transition_trace (t ▶ Event n v) (t' ▶ left_req)
-  | equiv_right_ack t t' n v :
-    event_trace_equiv_transition_trace t t' ->
-    n = ack (latch_output l) ->
-    event_trace_equiv_transition_trace (t ▶ Event n v) (t' ▶ right_ack)
-  | equiv_right_req t t' n v :
-    event_trace_equiv_transition_trace t t' ->
-    n = req (latch_output l) ->
-    event_trace_equiv_transition_trace (t ▶ Event n v) (t' ▶ right_req)
-  | equiv_clk_rise t t' n :
-    event_trace_equiv_transition_trace t t' ->
-    n = latch_clk l ->
-    event_trace_equiv_transition_trace (t ▶ Event n Bit1) (t' ▶ clk_rise)
-  | equiv_clk_fall t t' n v :
-    event_trace_equiv_transition_trace t t' ->
-    n = latch_clk l ->
-    event_trace_equiv_transition_trace (t ▶ Event n v) (t' ▶ clk_fall)
-*)
+
   | equiv_t_cons t t' e e' :
     event_equiv_transition_trace t t' ->
     Some e' = event_to_transition e ->
     event_equiv_transition_trace (t ▶ e) (t' ▶ e')
-
-  | equiv_event_hidden t t' x v :
-    event_equiv_transition_trace t t' ->
-    x ∉ from_list visible_domain ->
-    event_equiv_transition_trace (t ▶ Event x v) t'
   .
+
 
 
   Inductive state_equiv_marking : state name ->
                                   tail_list (event name value) ->
-                                  marking stage_MG ->
+                                  marking (stage_MG in_flag out_flag) ->
                                   tail_list token_transition ->
                                   Prop :=
   | state_equiv_marking0 (σ : state name) m : 
     σ = σR l false ->
-    m = init_marking stage_MG ->
+    m = init_marking (stage_MG in_flag out_flag) ->
     state_equiv_marking σ t_empty m t_empty
 
   | state_equiv_marking_step σ σ' t t' (e : token_transition) (e' : event name value) m m':
     state_equiv_marking σ t m t' ->
-    is_enabled stage_MG e m ->
+    is_enabled (stage_MG in_flag out_flag) e m ->
     e' = transition_to_event e σ ->
     σ' = update_event σ e' ->
-    m' = fire e stage_MG m ->
+    m' = fire e (stage_MG in_flag out_flag) m ->
     state_equiv_marking σ' (t ▶ e') m' (t' ▶ e)
 
   | state_equiv_marking_epsilon σ σ' t t' m :
@@ -209,7 +217,6 @@ Section TokenMG.
     σ' = update_event σ (Event x v) ->
     x ∉ from_list visible_domain ->
     state_equiv_marking σ' (t ▶ Event x v) m t'
-
   .
 
   Definition state_MG_traces : Ensemble (tail_list (event name value)) :=
@@ -219,7 +226,7 @@ Section TokenMG.
   Lemma stage_implies_stage_MG_event : forall σ t m e σ' t',
     state_equiv_marking σ t m t' ->
     latch_stage l ⊢ σ →{Some (transition_to_event e σ)} Some σ' ->
-    is_enabled stage_MG e m.
+    is_enabled (stage_MG in_flag out_flag) e m.
   Admitted.
 
 
@@ -235,7 +242,7 @@ Section TokenMG.
 
   Lemma event_equiv_transition_implies_state_equiv_marking : forall σ' t t' m,
     latch_stage l ⊢ σR l false →*{t} Some σ' ->
-    [stage_MG]⊢ t' ↓ m ->
+    [stage_MG in_flag out_flag]⊢ t' ↓ m ->
     event_equiv_transition_trace t t' ->
     state_equiv_marking σ' t m t'.
   Proof.
@@ -253,12 +260,10 @@ Section TokenMG.
       constructor; auto.
     * specialize (IHHstep _ eq_refl eq_refl).
       inversion Hequiv; subst.
-      + inversion HMG; subst.
-        eapply state_equiv_marking_step; eauto.
-        { admit (* true *). }
-        { admit (* true, but harder to show *). }
-      + eapply state_equiv_marking_internal; auto.
-        { admit (* true, I think *). }
+      inversion HMG; subst.
+      eapply state_equiv_marking_step; eauto.
+      { admit (* true *). }
+      { admit (* true, but harder to show *). }
     * specialize (IHHstep _ eq_refl eq_refl).
       eapply state_equiv_marking_epsilon; eauto.
       { admit (* true *). }
@@ -294,7 +299,7 @@ Admitted.
 
   Theorem stage_implies_stage_MG_traces : forall t σ',
     latch_stage l ⊢ σR l false →*{t} Some σ' ->
-    exists m t', event_equiv_transition_trace t t' /\ ([stage_MG]⊢ t' ↓ m).
+    exists m t', event_equiv_transition_trace t t' /\ ([stage_MG in_flag out_flag]⊢ t' ↓ m).
   Proof.
     intros t σ' Hstep.
     remember (latch_stage l) as S.
@@ -302,7 +307,7 @@ Admitted.
     generalize dependent HeqS.
     generalize dependent σ'.
     induction Hstep; intros σ'' Heqτ HeqS; try inversion Heqτ; subst; try clear Heqτ.
-    * exists (init_marking stage_MG).
+    * exists (init_marking (stage_MG in_flag out_flag)).
       exists t_empty.
       split; constructor.
     * specialize (IHHstep _ eq_refl eq_refl).
@@ -311,7 +316,7 @@ Admitted.
 
       destruct (In_Dec (from_list visible_domain) x) as [Hin | Hnin].
       + destruct (visible_domain_is_transition _ v Hin) as [e He].
-        assert (is_enabled stage_MG e m).
+        assert (is_enabled (stage_MG in_flag out_flag) e m).
         { eapply stage_implies_stage_MG_event.
           { apply event_equiv_transition_implies_state_equiv_marking; eauto. }
             
@@ -319,19 +324,24 @@ Admitted.
             eapply transition_step_value; eauto.
           }
         }
-        exists (fire e stage_MG m).
+        exists (fire e (stage_MG in_flag out_flag) m).
         exists (t' ▶ e).
         split.
         { constructor; auto.
         }
         { econstructor; eauto. }
-      + exists m. exists t'. split; auto.
-        apply equiv_event_hidden; auto.
+      + (* contradiction *)
+        contradict H1. admit.
     * clear H2. specialize (IHHstep _ eq_refl eq_refl).
       destruct IHHstep as [m [t' [Hequiv HMG]]].
       exists m. exists t'. split; auto.
-  Qed.
+  Admitted.
         
 
-  End TokenMG.
+  End SS_to_TokenMG.
+
+
+  Section Composition.
+
+  End Composition.
 End ClickMG.
