ClickRefinement.v
@@ -1,0 +1,135 @@
+Require Import Base.
+Require Import Circuit.
+Require Import StateSpace.
+Require Import Monad.
+
+Require Import List.
+Import ListNotations.
+Open Scope list_scope.
+
+Require Import MarkedGraph.
+Require Import Click.
+
+Import EnsembleNotation.
+Open Scope ensemble_scope.
+Require Import Coq.Program.Equality.
+
+Section MG_to_SS.
+
+  Print Marked
+
+End MG_to_SS.
+
+Section ClickRefinement.
+
+Variable name : Set.
+Context `{name_dec : eq_dec name}.
+Variable even odd : Set.
+Context `{scheme : naming_scheme name even odd}.
+
+Variable l : latch even odd.
+
+(** Define a state space [latch_stage_refinement such that every trace accepted
+by [latch_stage l] is also accepted by [latch_stage_refinement l] *)
+
+Print StateSpace. Print naming_scheme.
+Require Import ClickMG. 
+Class extended_naming_scheme :=
+    {place_name : forall {t1 t2 : token_transition}, stage_place t1 t2 -> name}.
+Context `{extended_naming_scheme}.
+Print stage_place.
+Definition name_is_place_dec : forall x,
+                          {t1 : token_transition &
+                           {t2 : token_transition & {p : stage_place t1 t2 & x = place_name p}}}
+                        + {forall t1 t2 (p : stage_place t1 t2), x <> place_name p}.
+Proof.
+  intros x. Print stage_place.
+
+  Ltac compare_place_name x p :=
+    compare x (place_name p);
+      [ left; do 3 eexists; reflexivity | ].
+  compare_place_name x left_ack_left_req.
+  compare_place_name x clk_fall_left_req.
+  compare_place_name x right_req_left_req.
+  compare_place_name x clk_rise_left_ack.
+  compare_place_name x clk_rise_right_req.
+  compare_place_name x right_req_right_ack.
+  compare_place_name x clk_fall_right_ack.
+  compare_place_name x left_ack_right_ack.
+  compare_place_name x clock_fall.
+  compare_place_name x left_req_clk_rise.
+  compare_place_name x right_ack_clk_rise.
+  right. intros t1 t2 p; destruct p; auto.
+Defined.
+
+
+Definition places_set : Ensemble name :=
+  fun x => exists t1 t2 (p : stage_place t1 t2), x = place_name p.
+
+
+
+Definition state_to_marking (σ : state name) : marking stage_MG :=
+  fun t1 t2 p => val_to_nat (σ (place_name p)).
+Print naming_scheme. Print token_transition.
+Print stage_MG. Print stage_place. Print value. Print enumerate.
+Arguments enumerate A {enumerable}.
+Print sig.
+  
+
+(** A transition should only fire if the caller has independently checked that it
+  is enabled. *) Print sigT. Print sumor.
+Search eq_dec token_transition.
+Existing Instance token_transition_eq_dec.
+Program Definition fire_in_state (t : token_transition) (σ : state name) : state name :=
+  fun x =>
+    match name_is_place_dec x with
+    (* if x is not a place, do nothign *)
+    | inright _ => σ x
+    | inleft (existT _ tin (existT _ tout (existT _ p x_is_p))) =>
+      (* corner case: do nothing *)
+      if tin =? tout then σ x
+      (* if x is a place leading into t, increment the value *)
+      else if t =? tout then dec_value (σ x)
+      (* if x is a place leading out of t, decrement the value *)
+      else if t =? tin then inc_value (σ x)
+      (* otherwise do nothing *)
+      else σ x
+    end.
+
+Print transition_name.
+Arguments transition_name {name even odd H0}.
+
+
+Inductive latch_step_refinement
+  : state name -> option (event name value) -> option (state name) -> Prop :=
+
+| transition_enabled σ σ' x v (t : token_transition) :
+  x = transition_name l t ->
+  is_enabled stage_MG t (state_to_marking σ) ->
+  v = transition_update_value t (σ x) ->
+  σ' = update (fire_in_state t σ) x v ->
+  latch_step_refinement σ (Some (Event x v)) (Some σ')
+
+| input_not_enabled σ x v t :
+  x ∈ space_input (latch_stage l) ->
+  x = transition_name l t ->
+  ~ is_enabled stage_MG t (state_to_marking σ) ->
+  latch_step_refinement σ (Some (Event x v)) None
+.
+
+
+
+(** the internal wires are all the wire names corresponding to places in the
+marked graph *)
+
+
+
+Definition latch_state_refinement : StateSpace name :=
+  {| space_input := space_input (latch_stage l)
+   ; space_output := space_output (latch_stage l)
+   ; space_internal := places_set 
+   ; space_step := latch_step_refinement
+   |}.
+
+
+End ClickRefinement.
